\documentclass[12pt]{article}

\usepackage{amsmath}

\begin{document}
	\begin{equation*}
		\cfrac{y^{n + 1} - 2y^{n} + y^{n - 1}}{\tau^{2}} + \omega^{2} y^{n} = f(n\tau)
		\Rightarrow
	\end{equation*}

	\begin{equation*}
		y^{n + 1} = (2 - \tau^{2} \omega^{2})y^{n} - y^{n - 1} + \tau^{2}f(n\tau)
	\end{equation*}

	\begin{equation*}
		\cfrac{y^{1} - y^{-1}}{2\tau} = V
		\Rightarrow 
		y^{-1} = y^{1} - 2\tau V
	\end{equation*}

	\begin{equation*}
		y^{1} = (2 - \tau^2 \omega^2) \cfrac{U}{2} + \tau V + \cfrac{\tau^{2}}{2}f(0)
	\end{equation*}

\end{document}
