\documentclass[12pt]{article}

\usepackage{amsmath}


\begin{document}
	\section{}
	\begin{equation*}
		u(0 + \tau) = u(0) + \tau u'(0) + \cfrac{\tau^2}{2!}u''(0) + O(\tau^3)
	\end{equation*}

	\begin{equation*}
		u''(t) + {\omega}^2u(t) = 0
		\Rightarrow
		u''(0) + {\omega}^2u(0) = 0
		\Rightarrow
		u''(0) =  -{\omega}^2u(0)
	\end{equation*}

	\begin{equation*}
		u'(0) = 0
	\end{equation*}

	\begin{equation*}
		u(0 + \tau) = u(0) - \cfrac{\tau^2}{2!}{\omega}^2u(0)
	\end{equation*}

	\section{}

	\begin{equation*}
		\cfrac{y^{1}  - y^{-1}}{2\tau} = V
		\Rightarrow
		y^{-1} = y^{1} - 2V\tau
	\end{equation*}

	\begin{equation*}
		y^{n + 1} = 2y^{n} - \tau^2\omega^2y^{n} - y^{n - 1}
	\end{equation*}

	\begin{equation*}
		n = 0 \Rightarrow y^{1} = 2y^{0} - \tau^2\omega^2y^{0} - y^{-1}
		\Rightarrow
		2y^{1} = U(2 - \tau^2\omega^2) + 2V\tau
	\end{equation*}

	\section{}
	\begin{equation*}
		u(0 + \tau) = u(0) + \tau u'(0) + \cfrac{\tau^2}{2!}u''(0) + O(\tau^3)
	\end{equation*}

	\begin{equation*}
		y^{1} = U + \tau V - \cfrac{\tau^2\omega^2}{2!}U + O(\tau^3)
	\end{equation*}
\end{document}
